consistently rename X to A and tc to cmp (#49)
* consistently rename X to A

* start renaming tc to cmp and use Generalizable Variables for typeclasses

* consistenly rename tc to cmp

* removed Generalizable Variables

Co-authored-by: Paul Cadman <pcadman@gmail.com>

comparable.v
@@ -3,28 +3,28 @@ Set Asymmetric Patterns.
 
 Require Import List.
 
-Class comparable (X : Type) :=
-  { compare : X -> X -> comparison (* Eq | Lt | Gt *)
+Class comparable (A : Type) :=
+  { compare : A -> A -> comparison (* Eq | Lt | Gt *)
 
   ; proof_compare_eq_is_equal
-    : forall (x y: X)
+    : forall (x y: A)
              (p: compare x y = Eq)
     , x = y
   ; proof_compare_eq_reflex
-    : forall (x: X)
+    : forall (x: A)
     , compare x x = Eq
   ; proof_compare_eq_trans
-    : forall (x y z: X)
+    : forall (x y z: A)
              (p: compare x y = Eq)
              (q: compare y z = Eq)
     , compare x z = Eq
   ; proof_compare_lt_assoc
-    : forall (x y z: X)
+    : forall (x y z: A)
              (p: compare x y = Lt)
              (q: compare y z = Lt)
     , compare x z = Lt
   ; proof_compare_gt_assoc
-    : forall (x y z: X)
+    : forall (x y z: A)
              (p: compare x y = Gt)
              (q: compare y z = Gt)
     , compare x z = Gt
@@ -45,14 +45,14 @@ Ltac compare_to_eq :=
   end.
 
 Lemma test_tactic_compare_to_eq
-  : forall {X: Type}
-           {tc: comparable X}
-           (x y: X)
+  : forall {A: Type}
+           {cmp: comparable A}
+           (x y: A)
            (p: Eq = compare x y),
   x = y.
 Proof.
 intros.
-set (Heq := tc).
+set (Heq := cmp).
 compare_to_eq.
 reflexivity.
 Qed.
@@ -83,9 +83,9 @@ Ltac induction_on_compare :=
 .
 
 Theorem proof_compare_eq_symm
-  : forall {X: Type}
-           {tc: comparable X}
-           (x y: X)
+  : forall {A: Type}
+           {cmp: comparable A}
+           (x y: A)
            (p: compare x y = Eq)
   , compare y x = Eq.
 Proof.
@@ -98,9 +98,9 @@ assumption.
 Qed.
 
 Theorem compare_eq_is_only_equal
-  : forall {X: Type}
-           {tc: comparable X}
-           (x1 x2: X)
+  : forall {A: Type}
+           {cmp: comparable A}
+           (x1 x2: A)
            (p: compare x1 x2 = compare x2 x1)
   , compare x1 x2 = Eq.
 Proof.
@@ -120,9 +120,9 @@ induction_on_compare.
 Qed.
 
 Theorem compare_lt_not_symm_1
-  : forall {X: Type}
-           {tc: comparable X}
-           (x1 x2: X)
+  : forall {A: Type}
+           {cmp: comparable A}
+           (x1 x2: A)
            (c12: compare x1 x2 = Lt)
            (c21: compare x2 x1 = Lt)
   , False.
@@ -135,9 +135,9 @@ discriminate.
 Qed.
 
 Theorem compare_lt_not_symm_2
-  : forall {X: Type}
-           {tc: comparable X}
-           (x1 x2: X)
+  : forall {A: Type}
+           {cmp: comparable A}
+           (x1 x2: A)
            (c12: compare x1 x2 = Lt)
            (c21: compare x2 x1 = Lt)
   , False.
@@ -151,9 +151,9 @@ discriminate.
 Qed.
 
 Theorem compare_gt_not_symm
-  : forall {X: Type}
-           {tc: comparable X}
-           (x1 x2: X)
+  : forall {A: Type}
+           {cmp: comparable A}
+           (x1 x2: A)
            (c12: compare x1 x2 = Gt)
            (c21: compare x2 x1 = Gt)
   , False.
@@ -167,9 +167,9 @@ discriminate.
 Qed.
 
 Theorem compare_lt_gt_symm
-  : forall {X: Type}
-           {tc: comparable X}
-           (x1 x2: X)
+  : forall {A: Type}
+           {cmp: comparable A}
+           (x1 x2: A)
            (p: compare x1 x2 = Lt)
   , compare x2 x1 = Gt.
 Proof.
@@ -188,9 +188,9 @@ induction iH.
 Qed.
 
 Theorem compare_gt_lt_symm
-  : forall {X: Type}
-           {tc: comparable X}
-           (x1 x2: X)
+  : forall {A: Type}
+           {cmp: comparable A}
+           (x1 x2: A)
            (p: compare x1 x2 = Gt)
   , compare x2 x1 = Lt.
 Proof.
@@ -206,7 +206,7 @@ Proof.
     discriminate.
 Qed.
 
-Fixpoint comparable_list {X: Type} {tc: comparable X} (xs: list X) (ys: list X) : comparison :=
+Fixpoint comparable_list {A: Type} {cmp: comparable A} (xs: list A) (ys: list A) : comparison :=
   match xs with
   | nil => match ys with
       | nil => Eq
