sort.v
@@ -6,7 +6,7 @@ Require Import List.
 Require Import comparable.
 
 (* is_sorted is a property that says whether a list is sorted *)
-Fixpoint is_sorted {X: Type} {tc: comparable X} (xs: list X) : Prop :=
+Fixpoint is_sorted {A: Type} {cmp: comparable A} (xs: list A) : Prop :=
   match xs with
   | nil => True
   | (x'::xs') => match xs' with
@@ -20,10 +20,10 @@ Fixpoint is_sorted {X: Type} {tc: comparable X} (xs: list X) : Prop :=
   end.
 
 Lemma is_sorted_sufficient_cond
-  {X: Type}
-  {tc: comparable X}
-  (x x' : X)
-  (xs: list X):
+  {A: Type}
+  {cmp: comparable A}
+  (x x' : A)
+  (xs: list A):
   ((compare x x' = Lt) \/ (compare x x' = Eq)) ->
   (is_sorted (x'::xs)) ->
   is_sorted (x::x'::xs).
@@ -33,38 +33,38 @@ unfold is_sorted.
 destruct H; rewrite H; trivial.
 Qed.
 
-Inductive is_sorted' {X: Type} {tc: comparable X} : list X -> Prop :=
+Inductive is_sorted' {A: Type} {cmp: comparable A} : list A -> Prop :=
   | empty_sorted' : is_sorted' nil
-  | singleton_sorted' (x: X) : is_sorted' (x :: nil)
+  | singleton_sorted' (x: A) : is_sorted' (x :: nil)
   | lessthan_sorted'
-    (x: X)
-    (y: X)
+    (x: A)
+    (y: A)
     (c : compare x y = Lt)
-    (xs: list X)
+    (xs: list A)
     (s: is_sorted' (y :: xs))
     : is_sorted' (x :: y :: xs)
   | equal_sorted'
-    (x: X)
-    (y: X)
+    (x: A)
+    (y: A)
     (c : compare x y = Eq)
-    (xs: list X)
+    (xs: list A)
     (s: is_sorted' (y :: xs))
     : is_sorted' (x :: y :: xs)
 .
 
-Inductive is_sorted'' {X: Type} {tc: comparable X} : list X -> Prop :=
+Inductive is_sorted'' {A: Type} {cmp: comparable A} : list A -> Prop :=
   | empty_sorted'' : is_sorted'' nil
   | singleton_sorted'' : forall x, is_sorted'' (x :: nil)
   | lessthan_sorted''
-    : forall (x: X) (xs: list X),
-      (exists (y: X) (ys: list X),
+    : forall (x: A) (xs: list A),
+      (exists (y: A) (ys: list A),
       xs = (y :: ys)
       /\ compare x y = Lt)
       /\ is_sorted'' xs
       -> is_sorted'' (x :: xs)
   | equal_sorted''
-    : forall (x: X) (xs: list X),
-      (exists (y: X) (ys: list X),
+    : forall (x: A) (xs: list A),
+      (exists (y: A) (ys: list A),
       xs = (y :: ys)
       /\ compare x y = Eq)
       /\ is_sorted'' xs
@@ -72,10 +72,10 @@ Inductive is_sorted'' {X: Type} {tc: comparable X} : list X -> Prop :=
 .
 
 Lemma tail_of_is_sorted_is_sorted:
-  forall {X: Type}
-  {tc: comparable X}
-  (x: X)
-  (xs: list X),
+  forall {A: Type}
+  {cmp: comparable A}
+  (x: A)
+  (xs: list A),
   is_sorted (x :: xs) -> is_sorted xs.
 Proof.
 (* TODO: Good First Issue 
@@ -84,26 +84,26 @@ Proof.
 Admitted.
 
 Lemma tail_of_is_sorted'_is_sorted':
-  forall {X: Type}
-  {tc: comparable X}
-  (x: X)
-  (xs: list X),
+  forall {A: Type}
+  {cmp: comparable A}
+  (x: A)
+  (xs: list A),
   is_sorted' (x :: xs) -> is_sorted' xs.
 Proof.
 (* TODO: Good First Issue *)
 Admitted.
 
 Lemma tail_of_is_sorted''_is_sorted'':
-  forall {X: Type}
-  {tc: comparable X}
-  (x: X)
-  (xs: list X),
+  forall {A: Type}
+  {cmp: comparable A}
+  (x: A)
+  (xs: list A),
   is_sorted'' (x :: xs) -> is_sorted'' xs.
 Proof.
 (* TODO: Good First Issue *)
 Admitted.
 
-Theorem is_sorted_and_is_sorted'_are_equivalent : forall {X: Type} {tc: comparable X} (xs: list X),
+Theorem is_sorted_and_is_sorted'_are_equivalent : forall {A: Type} {cmp: comparable A} (xs: list A),
   is_sorted xs <-> is_sorted' xs.
 Proof.
 intros.
@@ -141,14 +141,14 @@ split.
 *)
 Admitted.
 
-Theorem is_sorted'_and_is_sorted''_are_equivalent : forall {X: Type} {tc: comparable X} (xs: list X),
+Theorem is_sorted'_and_is_sorted''_are_equivalent : forall {A: Type} {cmp: comparable A} (xs: list A),
   is_sorted' xs <-> is_sorted'' xs.
 Proof.
 (* TODO: Good First Issue *)
 Admitted.
 
 (* insert_sort is a helper function for sort *)
-Fixpoint insert_sort {X: Type} {tc: comparable X} (xs: list X) (x: X) : list X :=
+Fixpoint insert_sort {A: Type} {cmp: comparable A} (xs: list A) (x: A) : list A :=
   match xs with
   | nil => x :: nil
   | (x'::xs') => match compare x x' with
@@ -159,20 +159,20 @@ Fixpoint insert_sort {X: Type} {tc: comparable X} (xs: list X) (x: X) : list X :
   end.
 
 (* insert_sort_sorts is a helper lemma for sort_sorts *)
-Lemma insert_sort_sorts: forall {X: Type} {tc: comparable X} (xs: list X) (x: X) {s: is_sorted xs},
+Lemma insert_sort_sorts: forall {A: Type} {cmp: comparable A} (xs: list A) (x: A) {s: is_sorted xs},
   is_sorted (insert_sort xs x).
 Proof.
 (* TODO: Good First Issue *)
 Admitted.
 
 (* sort is a helper function for eval_list_sort *)
-Fixpoint sort {X: Type} {tc: comparable X} (xs: list X) : list X :=
+Fixpoint sort {A: Type} {cmp: comparable A} (xs: list A) : list A :=
   match xs with
   | nil => nil
   | (x'::xs') => insert_sort (sort xs') x'
   end.
 
-Theorem sort_sorts: forall {X: Type} {tc: comparable X} (xs: list X),
+Theorem sort_sorts: forall {A: Type} {cmp: comparable A} (xs: list A),
   is_sorted (sort xs).
 Proof.
 induction xs.
