reduce_orb.v
@@ -2,18 +2,24 @@ Require Import Bool.
 
 Ltac reduce_orb_step :=
   match goal with
-  | [ |- context [?A || ?B || (?C || ?B)]] =>
-    rewrite orb_comm with C B
-  | [ |- context [?A || ?B || (?B || ?C)]] =>
-    rewrite orb_assoc with (A||B) B C
-  | [ |- context [?A || ?B || ?B]] =>
-    rewrite <- orb_assoc with A B B
-  | [ |- context [?B || ?B]] =>
+  | [ |- context [?X || ?Y || (?Z || ?Y)]] =>
+    rewrite orb_comm with Z Y
+  | [ |- context [?X || ?Y || (?Y || ?Z)]] =>
+    rewrite orb_assoc with (X||Y) Y Z
+  | [ |- context [?X || ?Y || ?Y]] =>
+    rewrite <- orb_assoc with X Y Y
+  | [ |- context [?Y || ?Y]] =>
     rewrite orb_diag
-  | [|- context [?A || ?B || ?C = ?A || ?C || ?B]] =>
-    rewrite <- orb_assoc with A C B;
-    rewrite orb_comm with C B;
-    rewrite orb_assoc with A B C
+  | [|- context [?X || ?Y || ?Z = ?X || ?Z || ?Y]] =>
+    rewrite <- orb_assoc with X Z Y;
+    rewrite orb_comm with Z Y;
+    rewrite orb_assoc with X Y Z
   end.
 
 Ltac reduce_orb := repeat (try reduce_orb_step).
+
+(* TODO: Good First Issue
+   Add some examples of using reduce_orb_step, 
+   by creating theorems that are proved using reduce_orb_step
+   The theorem names should start with test_
+*)
